src/verification/semantics/stream_zero.lean
@@ -1,0 +1,44 @@
+import verification.semantics.skip_stream
+
+/-!
+
+# Zero stream
+
+In this file, we define the zero stream, which immediately terminates
+producing no output. This stream is important for defining
+a nested version of `add`, since `add` requires the value type to 
+have a `0`.
+
+## Main results
+All the results in this file are trivial (i.e. follow from `false.elim : false → C`)
+because the stream itself does not produce anything, and has no valid states.
+
+-/
+
+def Stream.zero (ι : Type) (α : Type*) : Stream ι α :=
+{ σ := unit,
+  valid := λ _, false,
+  ready := λ _, false,
+  skip := λ _, false.elim,
+  index := λ _, false.elim,
+  value := λ _, false.elim } 
+
+variables {ι : Type} [linear_order ι] {α β : Type*}
+
+instance : is_bounded (Stream.zero ι α) :=
+⟨⟨empty_relation, empty_wf, λ q, false.drec _⟩⟩
+
+@[simp] lemma Stream.zero_map (f : α → β) :
+  (Stream.zero ι α).map f = Stream.zero ι β :=
+by { ext; solve_refl, exfalso, assumption, }
+
+variables [add_zero_class α] 
+
+@[simp] lemma Stream.zero_eval :
+  (Stream.zero ι α).eval = 0 :=
+by { ext q i, rw Stream.eval_invalid, { simp, }, exact not_false, }
+
+instance : is_strict_lawful (Stream.zero ι α) :=
+{ mono := λ q, false.drec _,
+  skip_spec := λ q, false.drec _,
+  strict_mono := ⟨λ q, false.drec _, λ q, false.drec _⟩ }
